src/Analysis/Domains/Sign_Exec_Sound.thy
@@ -91,16 +91,31 @@ proof -
   have pp_st: "part_post_solution (side_cfg_T_ip_st g sign_tf_st bot cinit_sign_st)
                  (cfg_exit g) (snd sol) (fst sol)"
     using pp0 by (simp add: sign_exec_eqs_def g_def)
-  have pp_abs: "part_post_solution (side_cfg_T_ip g sign_tf (\<squnion>) bot (\<lambda>x. if is_global x then SZero else STop))
+  interpret se: sound_effectful_transfer gamma_sign sign_etf
+    by (rule sign_sound_etf)
+  have pp_eff: "part_post_solution
+                  (side_cfg_T_ip_eff g sign_etf bot
+                     (\<lambda>x. if is_global x then SZero else STop))
                   (cfg_exit g) \<sigma> (fst sol)"
-    using part_post_solution_st_to_abs[OF sign_tf_st_commute pp_st]
+    using part_post_solution_st_to_abs_eff[OF sign_tf_st_commute pp_st]
+    unfolding sign_etf_def
     by (simp add: \<sigma>_def fun_of_st_bot fun_of_st_cinit_sign_st bot_fun_def)
+  have ed: "\<And>b z \<sigma>'. Inl z \<in> dep_aux \<sigma>' (apply_etf sign_etf b z)"
+    unfolding sign_etf_def by (rule dep_aux_apply_etf_from_tf_src)
+  have cd1: "\<And>c2 e2 \<sigma>'. Inl c2 \<in> dep_aux \<sigma>' (etf_combine sign_etf c2 e2)"
+    unfolding sign_etf_def by (rule dep_aux_etf_combine_from_tf_call)
+  have cd2: "\<And>c2 e2 \<sigma>'. Inl e2 \<in> dep_aux \<sigma>' (etf_combine sign_etf c2 e2)"
+    unfolding sign_etf_def by (rule dep_aux_etf_combine_from_tf_exit)
+  have es: "\<And>a u. static_deps (apply_etf sign_etf a u)"
+    unfolding sign_etf_def by (rule static_deps_apply_etf_from_tf)
+  have cs: "\<And>cc ex. static_deps (etf_combine sign_etf cc ex)"
+    unfolding sign_etf_def by (rule static_deps_etf_combine_from_tf)
   have reach: "ip_reaches g (cfg_entry g) (cfg_exit g)"
     by (simp add: g_def compile_prog_entry_ip_reaches_exit)
   have entry_in: "cfg_entry g \<in> fst sol"
-    by (rule side_ip_cone_in_vars[OF pp_abs fin finC reach])
+    by (rule side_ip_cone_in_vars_eff[OF pp_eff fin finC ed cd1 cd2 es cs reach])
   have entry_le: "(\<lambda>x. if is_global x then SZero else STop) \<le> side_env \<sigma> (cfg_entry g)"
-    by (rule s0_le_side_env_entry_ip[OF pp_abs entry_in])
+    by (rule s0_le_side_env_entry_ip_eff[OF pp_eff entry_in])
   have seed_cov: "cinit_stores \<subseteq> sign_domain.gamma_state (\<lambda>x. if is_global x then SZero else STop)"
     unfolding cinit_stores_def sign_domain.gamma_state_def
     by (auto simp: gamma_sign.simps)
@@ -108,8 +123,8 @@ proof -
     using seed_cov sign_domain.gamma_state_mono[OF entry_le] by (rule subset_trans)
   have "cfg_collect_ip g cinit_stores (cfg_exit g)
         \<le> sign_domain.gamma_state (side_env \<sigma> (cfg_exit g))"
-    using sound_transfer.side_collect_sound_ip_exit_pruned
-            [OF sign_sound_tf.sound_transfer_axioms pp_abs fin finC entry_cov] .
+    by (rule se.side_collect_sound_ip_exit_pruned_eff
+          [OF pp_eff fin finC entry_cov ed cd1 cd2 es cs])
   then show ?thesis
     by (simp add: g_def \<sigma>_def sol_def sign_exec_def sign_exec_raw_def)
 qed
